better outlining

VCVio/CryptoFoundations/SymmEncAlg.lean
@@ -16,61 +16,39 @@ secret keys of type `K`, and ciphertext space `C`.
 
 open OracleSpec OracleComp OracleAlg BigOperators
 
-structure SymmEncAlg {ι : Type}
-    (spec : ℕ → OracleSpec ι) (M K C : ℕ → Type)
+structure SymmEncAlg {ι : Type} (spec : ℕ → OracleSpec ι) (M K C : ℕ → Type)
     extends OracleAlg spec where
   (keygen (sp : ℕ) : OracleComp (spec sp) (K sp))
-  (encrypt (sp : ℕ) : M sp → K sp → OracleComp (spec sp) (C sp))
-  (decrypt (sp : ℕ) : C sp → K sp → OracleComp (spec sp) (M sp))
+  (encrypt (sp : ℕ) : K sp → M sp → OracleComp (spec sp) (C sp))
+  (decrypt (sp : ℕ) : K sp → C sp → OracleComp (spec sp) (M sp))
 
 namespace SymmEncAlg
 
 variable {ι : Type} {spec : ℕ → OracleSpec ι} {M K C : ℕ → Type}
 
-section sound
+section isSound
 
 variable [Π sp, DecidableEq (M sp)]
 
-/-- Experiment for checking that a symmetric encryption algorithm is sound,
-i.e. that decryption properly reverses encryption -/
-@[simp]
-def soundnessExp (encAlg : SymmEncAlg spec M K C)
-    (mDist : (sp : ℕ) → OracleComp (spec sp) (M sp)) :
-    SecExp spec where
-  main := λ sp ↦ do
-    let m ← mDist sp
-    let k ← encAlg.keygen sp
-    let σ ← encAlg.encrypt sp m k
-    let m' ← encAlg.decrypt sp σ k
-    return m = m'
-  __ := encAlg
-
-/-- An asymmetric encryption algorithm is sound if messages always decrypt to themselves. -/
+/-- A symmetric encryption algorithm is sound is messages decrypt to themselves given a random key.
+Note that we assume the algorithm never fails, although in general this could be modified
+to allow for a (negligible) chance of encryption failure. -/
 def isSound (encAlg : SymmEncAlg spec M K C) : Prop :=
-  ∀ mDist, negligible (1 - (soundnessExp encAlg mDist).advantage)
+  ∀ sp : ℕ, ∀ m : M sp, [= m | do
+    let k ← encAlg.keygen sp
+    let σ ← encAlg.encrypt sp k m
+    encAlg.decrypt sp k σ] = 1
 
 variable (encAlg : SymmEncAlg spec M K C)
 
-@[simp]
-lemma isSound_iff_forall (encAlg : SymmEncAlg spec M K C) :
-    encAlg.isSound ↔ ∀ sp : ℕ, ∀ m : M sp, (encAlg.exec sp (do
-      let k ← encAlg.keygen sp
-      let σ ← encAlg.encrypt sp m k
-      encAlg.decrypt sp σ k)).support ⊆ {m} := by
-  sorry
-  -- refine forall_congr' (λ m ↦ ?_)
-  -- simp only [soundnessExp, @eq_comm _ m, bind_pure_comp, ← map_bind, SecExp.advantage_eq_one_iff,
-  --   exec_map, exec_bind, simulate'_bind, support_map,
-  -- support_bind, Set.mem_image, Set.mem_iUnion,
-  --   exists_prop, Prod.exists, decide_eq_false_iff_not, not_exists, not_and, not_not,
-  --   forall_exists_index, and_imp, Set.subset_singleton_iff]
+-- lemma isSound_iff_forall_mem_support :
 
-end sound
+end isSound
 
-section perfectSecrecy
+-- section perfectSecrecy
 
 
 
-end perfectSecrecy
+-- end perfectSecrecy
 
 end SymmEncAlg
